progs/verif_sha_final3.v
@@ -1,0 +1,525 @@
+Require Import floyd.proofauto.
+Require Import progs.sha.
+Require Import progs.SHA256.
+Require Import progs.spec_sha.
+Require Import progs.sha_lemmas.
+Require Import progs.sha_lemmas2.
+Require Import progs.verif_sha_final2.
+Local Open Scope logic.
+
+
+Definition sha_final_epilog :=
+  (Ssequence
+     (Scall None
+        (Evar _sha256_block_data_order
+           (Tfunction
+              (Tcons (tptr t_struct_SHA256state_st) (Tcons (tptr tvoid) Tnil))
+              tvoid))
+        [Etempvar _c (tptr t_struct_SHA256state_st),
+        Etempvar _p (tptr tuchar)])
+     (Ssequence
+        (Sassign
+           (Efield
+              (Ederef (Etempvar _c (tptr t_struct_SHA256state_st))
+                 t_struct_SHA256state_st) _num tuint)
+           (Econst_int (Int.repr 0) tint))
+        (Ssequence
+           (Ssequence
+              (Scall (Some _ignore'2)
+                 (Evar _memset
+                    (Tfunction
+                       (Tcons (tptr tvoid) (Tcons tint (Tcons tuint Tnil)))
+                       (tptr tvoid)))
+                 [Etempvar _p (tptr tuchar), Econst_int (Int.repr 0) tint,
+                 Ebinop Omul (Econst_int (Int.repr 16) tint)
+                   (Econst_int (Int.repr 4) tint) tint])
+              (Sset _ignore (Etempvar _ignore'2 (tptr tvoid))))
+           (Ssequence final_loop (Sreturn None))))).
+
+Lemma sha_final_part3:
+forall (Espec : OracleKind) (md c : val) (shmd : share)
+  (hashed lastblock: list int) msg
+ (Hshmd: writable_share shmd),
+ NPeano.divide LBLOCK (length hashed) ->
+ length lastblock = LBLOCK ->
+ generate_and_pad_msg msg = hashed++lastblock ->
+semax
+  (initialized _cNl
+     (initialized _cNh
+        (initialized _ignore (initialized _ignore'1 Delta_final_if1))))
+  (PROP  ()
+   LOCAL  (`(eq (offset_val (Int.repr 40) c)) (eval_id _p);
+   `(eq md) (eval_id _md); `(eq c) (eval_id _c))
+   SEP 
+   (`(data_block Tsh (intlist_to_Zlist lastblock)
+                 (offset_val (Int.repr 40) c));
+   `(array_at tuint Tsh
+       (ZnthV tuint (map Vint (process_msg init_registers hashed))) 0 8 c);
+   `(field_at_ Tsh t_struct_SHA256state_st _Nl c);
+   `(field_at_ Tsh t_struct_SHA256state_st _Nh c);
+   `(field_at_ Tsh t_struct_SHA256state_st _num c); K_vector;
+   `(memory_block shmd (Int.repr 32) md)))
+  sha_final_epilog
+  (function_body_ret_assert tvoid
+     (PROP  ()
+      LOCAL ()
+      SEP  (K_vector; `(data_at_ Tsh t_struct_SHA256state_st c);
+      `(data_block shmd (SHA_256 msg) md)))).
+Proof.
+intros.
+unfold sha_final_epilog.
+forward. (* sha256_block_data_order (c,p); *)
+instantiate (1:= (hashed, lastblock, c, (offset_val (Int.repr 40) c), Tsh))
+  in (Value of witness).
+entailer!.
+ erewrite K_vector_globals by (split3; [eassumption | reflexivity.. ]).
+cancel.
+normalize.
+replace_SEP 0%Z  (`(array_at tuint Tsh
+          (tuints
+             (process_msg init_registers (hashed ++ lastblock))) 0 8 c) *
+      `(at_offset 40 (array_at tuchar Tsh (ZnthV tuchar []) 0 64) c) *
+      K_vector).
+entailer!.
+ erewrite K_vector_globals by (split3; [eassumption | reflexivity.. ]).
+cancel.
+unfold data_block.
+rewrite array_at_ZnthV_nil.
+rewrite Zlength_correct.
+rewrite length_intlist_to_Zlist.
+rewrite H0.
+change (Z.of_nat (4 * LBLOCK))%Z with 64%Z.
+unfold at_offset.
+apply array_at__array_at.
+normalize.
+rewrite <- H1.
+forward. (* c->num=0; *)
+forward. (* ignore=memset (p,0,SHA_CBLOCK); *)
+instantiate (1:= (Tsh, (offset_val (Int.repr 40) c), 64%Z, Int.zero))
+  in (Value of witness).
+entailer!.
+ rewrite (memory_block_array_tuchar _ 64%Z) by Omega1.
+pull_left (at_offset 40 (array_at tuchar Tsh (ZnthV tuchar []) 0 64) c).
+repeat rewrite sepcon_assoc; apply sepcon_derives; [ | cancel].
+unfold at_offset.
+cancel.
+autorewrite with subst.
+replace_SEP 0%Z (`(array_at tuchar Tsh (fun _ : Z => Vint Int.zero) 0 64
+          (offset_val (Int.repr 40) c))).
+entailer!.
+forward.  (* ignore = ignore'; *)
+fold t_struct_SHA256state_st.
+pose proof (length_process_msg (generate_and_pad_msg msg)).
+replace Delta with
+ (initialized _ignore'2 (initialized _cNl (initialized _cNh (initialized _ignore (initialized _ignore'1 Delta_final_if1)))))
+ by (simplify_Delta; reflexivity).
+eapply semax_pre; [ | apply final_part4; auto].
+entailer!.
+Qed.
+
+Lemma final_part5:
+forall (hashed dd hashed' dd' : list int) (pad : Z) (hi' lo' : list Z)
+  (hi lo : int) c_,
+(* (pad=0%Z \/ dd'=nil) -> *)
+NPeano.divide LBLOCK (length hashed) ->
+(length dd < CBLOCK)%nat ->
+(Zlength dd < 64)%Z ->
+(length (map Int.unsigned dd') + 8 <= CBLOCK)%nat ->
+(0 <= pad < 8)%Z ->
+NPeano.divide LBLOCK (length hashed') ->
+intlist_to_Zlist hashed' ++ map Int.unsigned dd' =
+intlist_to_Zlist hashed ++
+map Int.unsigned dd ++ [128%Z] ++ map Int.unsigned (zeros pad) ->
+length hi' = 4%nat ->
+length lo' = 4%nat ->
+isptr c_ ->
+hi' = intlist_to_Zlist [hi] /\ lo' = intlist_to_Zlist [lo] ->
+array_at tuchar Tsh (ZnthV tuchar (map Vint (map Int.repr lo'))) 0 4
+  (offset_val (Int.repr 100) c_) *
+array_at tuchar Tsh (ZnthV tuchar (map Vint (map Int.repr hi'))) 0 4
+  (offset_val (Int.repr 96) c_) *
+array_at tuchar Tsh (fun _ : Z => Vint Int.zero) 0
+  (Z.of_nat CBLOCK - 8 - Zlength dd')
+  (offset_val (Int.repr (Zlength dd' + 40)) c_) *
+array_at tuchar Tsh (ZnthV tuchar (map Vint dd')) 0 (Zlength dd')
+  (offset_val (Int.repr 40) c_)
+|-- array_at tuchar Tsh
+      (ZnthV tuchar
+         (map Vint
+            (dd' ++
+             zeros (Z.of_nat CBLOCK - 8 - Zlength dd') ++
+             map Int.repr (hi' ++ lo')))) 0 64 (offset_val (Int.repr 40) c_).
+Proof.
+intros until c_.
+intros H4 H3 H3' H0 H1 H2 H5 Lhi Llo Pc_ Hhilo.
+ rewrite (split_array_at (Zlength dd') tuchar Tsh _ 0 64)
+  by (clear - H0; rewrite Zlength_correct; change CBLOCK with 64%nat in H0;
+  rewrite map_length in H0; omega).
+ rewrite (split_array_at 56 tuchar Tsh _ (Zlength dd') 64)
+  by (clear - H0; rewrite Zlength_correct; change CBLOCK with 64%nat in H0;
+  rewrite map_length in H0; omega).
+ rewrite (split_array_at 60 tuchar Tsh _ 56 64) by omega.
+ replace (offset_val (Int.repr 100) c_) with
+            (offset_val (Int.repr (sizeof tuchar * 60)) (offset_val (Int.repr 40) c_))
+  by (rewrite offset_offset_val; destruct c_; reflexivity).
+ replace (offset_val (Int.repr 96) c_) with
+            (offset_val (Int.repr (sizeof tuchar * 56)) (offset_val (Int.repr 40) c_))
+  by (rewrite offset_offset_val; destruct c_; reflexivity).
+ replace (offset_val (Int.repr (Zlength dd' + 40)) c_) with
+            (offset_val (Int.repr (sizeof tuchar * Zlength dd')) (offset_val (Int.repr 40) c_))
+  by (change (sizeof tuchar) with 1%Z; rewrite Z.mul_1_l; rewrite offset_offset_val; rewrite Int.add_commut, add_repr; reflexivity).
+ forget (offset_val (Int.repr 40) c_) as cc.
+ repeat rewrite <- offset_val_array_at.
+ apply derives_trans with
+  (array_at tuchar Tsh (ZnthV tuchar (map Vint dd')) 0 (Zlength dd') cc *
+   array_at tuchar Tsh (fun _ : Z => Vint Int.zero) (Zlength dd' + 0)
+   (Zlength dd' + (Z.of_nat CBLOCK - 8 - Zlength dd')) cc *
+   array_at tuchar Tsh (fun i : Z => ZnthV tuchar (map Vint (map Int.repr hi')) (i - 56)) 
+      56 60 cc *
+  array_at tuchar Tsh (fun i : Z => ZnthV tuchar (map Vint (map Int.repr lo')) (i - 60)) 
+      60 64 cc);
+  [solve [cancel] | ].
+ rewrite Z.add_0_r.
+ replace (Zlength dd' + (Z.of_nat CBLOCK - 8 - Zlength dd'))%Z
+  with 56%Z by (change (Z.of_nat CBLOCK) with 64%Z; clear; omega).
+ assert (Zlength dd' >= 0)%Z by (rewrite Zlength_correct; omega).
+ assert (Zlength dd' = Z.of_nat (length (map Vint dd'))).
+ rewrite Zlength_correct, map_length; reflexivity.
+ assert (Z.of_nat CBLOCK - 8 - Z.of_nat (length dd') >= 0)%Z.
+    clear - H0; admit. (* tedious *)
+ repeat rewrite sepcon_assoc;
+ repeat apply sepcon_derives; apply derives_refl';
+ apply equal_f; try apply array_at_ext; intros;
+ unfold ZnthV; repeat rewrite if_false by omega.
++ repeat rewrite map_app.
+   rewrite app_nth1; [reflexivity | ].
+ apply Nat2Z.inj_lt. rewrite Z2Nat.id by omega; omega.
++ repeat rewrite map_app.
+   rewrite app_nth2. rewrite app_nth1.
+  rewrite nth_map_zeros. auto.
+  rewrite Nat2Z.inj_sub by Omega1. Omega1.
+  rewrite (map_length _ (zeros _)).
+  rewrite length_zeros.
+  apply Nat2Z.inj_lt; rewrite Nat2Z.inj_sub; Omega1.
+  Omega1.
++ repeat rewrite map_app.
+   rewrite <- app_ass.
+   rewrite app_nth2. rewrite app_nth1.
+   f_equal.    rewrite app_length.  
+   repeat rewrite map_length; rewrite map_length in H6.
+   rewrite length_zeros.
+   rewrite H6. Omega1.
+  rewrite app_length; rewrite (map_length _ (zeros _)); rewrite length_zeros.
+  rewrite H6. repeat rewrite map_length.
+  rewrite Lhi.
+    change (Z.of_nat CBLOCK - 8)%Z with 56%Z. 
+  apply Nat2Z.inj_lt; try omega.
+  rewrite Nat2Z.inj_sub; try Omega1.
+  rewrite H6; repeat rewrite app_length; repeat rewrite map_length;
+   rewrite length_zeros.
+  Omega1.
++ admit.  (* tedious *)
+Qed.
+
+Lemma final_part2:
+forall (Espec : OracleKind) (hashed : list int) (md c : val) (shmd : share),
+writable_share shmd ->
+name _md ->
+name _c ->
+name _p ->
+name _n ->
+name _cNl ->
+name _cNh ->
+name _ignore ->
+forall (hi lo : int) (dd : list int),
+NPeano.divide LBLOCK (length hashed) ->
+((Zlength hashed * 4 + Zlength dd)*8)%Z = hilo hi lo ->
+(length dd < CBLOCK)%nat ->
+(Zlength dd < 64)%Z ->
+forall (hashed' dd' : list int) (pad : Z),
+ (pad=0%Z \/ dd'=nil) ->
+(length (map Int.unsigned dd') + 8 <= CBLOCK)%nat ->
+(0 <= pad < 8)%Z ->
+NPeano.divide LBLOCK (length hashed') ->
+intlist_to_Zlist hashed' ++ map Int.unsigned dd' =
+intlist_to_Zlist hashed ++
+map Int.unsigned dd ++ [128%Z] ++ map Int.unsigned (zeros pad) ->
+forall p0 : val,
+semax (initialized _ignore (initialized _ignore'1 Delta_final_if1))
+  (PROP  ()
+   LOCAL 
+   (`(eq (force_val (sem_add_pi tuchar p0 (Vint (Int.repr (16 * 4 - 8))))))
+      (eval_id _p); `(eq (Vint (Int.repr (Zlength dd')))) (eval_id _n);
+   `(eq p0) (`(offset_val (Int.repr 40)) (`force_ptr (eval_id _c)));
+   `(eq md) (eval_id _md); `(eq c) (eval_id _c))
+   SEP 
+   (`(array_at tuchar Tsh (fun _ : Z => Vint Int.zero) 0
+        (Z.of_nat CBLOCK - 8 - Zlength dd')
+        (offset_val (Int.repr (40 + Zlength dd')) c));
+   `(array_at tuint Tsh
+       (ZnthV tuint (map Vint (process_msg init_registers hashed'))) 0 8 c);
+   `(field_at Tsh t_struct_SHA256state_st _Nl (Vint lo) c);
+   `(field_at Tsh t_struct_SHA256state_st _Nh (Vint hi) c);
+   `(array_at tuchar Tsh (ZnthV tuchar (map Vint dd')) 0 (Zlength dd')
+       (offset_val (Int.repr 40) c));
+   `(array_at tuchar Tsh (ZnthV tuchar (map Vint dd')) (Z.of_nat CBLOCK - 8)
+       64 (offset_val (Int.repr 40) c));
+   `(field_at_ Tsh t_struct_SHA256state_st _num c); K_vector;
+   `(memory_block shmd (Int.repr 32) md)))
+  (Ssequence
+     (Sset _cNh
+        (Efield
+           (Ederef (Etempvar _c (tptr t_struct_SHA256state_st))
+              t_struct_SHA256state_st) _Nh tuint))
+     (Ssequence
+        (Ssequence
+           (Scall None
+              (Evar ___builtin_write32_reversed
+                 (Tfunction (Tcons (tptr tuint) (Tcons tuint Tnil)) tvoid))
+              [Ecast (Etempvar _p (tptr tuchar)) (tptr tuint),
+              Etempvar _cNh tuint])
+           (Sset _p
+              (Ebinop Oadd (Etempvar _p (tptr tuchar))
+                 (Econst_int (Int.repr 4) tint) (tptr tuchar))))
+        (Ssequence
+           (Sset _cNl
+              (Efield
+                 (Ederef (Etempvar _c (tptr t_struct_SHA256state_st))
+                    t_struct_SHA256state_st) _Nl tuint))
+           (Ssequence
+              (Ssequence
+                 (Scall None
+                    (Evar ___builtin_write32_reversed
+                       (Tfunction (Tcons (tptr tuint) (Tcons tuint Tnil))
+                          tvoid))
+                    [Ecast (Etempvar _p (tptr tuchar)) (tptr tuint),
+                    Etempvar _cNl tuint])
+                 (Sset _p
+                    (Ebinop Oadd (Etempvar _p (tptr tuchar))
+                       (Econst_int (Int.repr 4) tint) (tptr tuchar))))
+              (Ssequence
+                 (Sset _p
+                    (Ebinop Osub (Etempvar _p (tptr tuchar))
+                       (Ebinop Omul (Econst_int (Int.repr 16) tint)
+                          (Econst_int (Int.repr 4) tint) tint) (tptr tuchar)))
+                 (Ssequence
+                    (Scall None
+                       (Evar _sha256_block_data_order
+                          (Tfunction
+                             (Tcons (tptr t_struct_SHA256state_st)
+                                (Tcons (tptr tvoid) Tnil)) tvoid))
+                       [Etempvar _c (tptr t_struct_SHA256state_st),
+                       Etempvar _p (tptr tuchar)])
+                    (Ssequence
+                       (Sassign
+                          (Efield
+                             (Ederef
+                                (Etempvar _c (tptr t_struct_SHA256state_st))
+                                t_struct_SHA256state_st) _num tuint)
+                          (Econst_int (Int.repr 0) tint))
+                       (Ssequence
+                          (Ssequence
+                             (Scall (Some _ignore'2)
+                                (Evar _memset
+                                   (Tfunction
+                                      (Tcons (tptr tvoid)
+                                         (Tcons tint (Tcons tuint Tnil)))
+                                      (tptr tvoid)))
+                                [Etempvar _p (tptr tuchar),
+                                Econst_int (Int.repr 0) tint,
+                                Ebinop Omul (Econst_int (Int.repr 16) tint)
+                                  (Econst_int (Int.repr 4) tint) tint])
+                             (Sset _ignore (Etempvar _ignore'2 (tptr tvoid))))
+                          (Ssequence
+                             final_loop
+                             (Sreturn None))))))))))
+  (function_body_ret_assert tvoid
+     (PROP  ()
+      LOCAL ()
+      SEP  (K_vector; `(data_at_ Tsh t_struct_SHA256state_st c);
+      `(data_block shmd
+          (intlist_to_Zlist
+             (process_msg init_registers
+                (generate_and_pad_msg
+                   (intlist_to_Zlist hashed ++ map Int.unsigned dd))))
+          md)))).
+Proof.
+ intros Espec hashed md c shmd H md_ c_ p n cNl cNh ignore
+ hi lo dd H4 H7 H3 H3' hashed' dd' pad PAD H0 H1 H2 H5 p0.
+ pose (hibytes := Basics.compose force_int (ZnthV tuchar (map Vint (map Int.repr (intlist_to_Zlist [hi]))))).
+ pose (lobytes := Basics.compose force_int (ZnthV tuchar (map Vint (map Int.repr (intlist_to_Zlist [lo]))))).
+ rewrite (split_array_at 60%Z tuchar Tsh _ (Z.of_nat CBLOCK - 8)%Z 64%Z)
+  by (change (Z.of_nat CBLOCK) with 64%Z; split; computable).
+ forward. (* cNh=c->Nh; *)
+ forward. (* (void)HOST_l2c(cNh,p); *)
+ instantiate (1:=(offset_val (Int.repr 56) (offset_val (Int.repr 40) c),
+                         Tsh, hibytes)) in (Value of witness).
+ rewrite (Z.add_comm 40).
+ entailer!.
+ destruct c; try (contradiction Pc); simpl. f_equal; rewrite Int.add_assoc; rewrite mul_repr; rewrite add_repr; reflexivity.
+ unfold hibytes.
+ symmetry; rewrite (nth_big_endian_integer 0 [hi] hi) at 1 by reflexivity.
+ f_equal; extensionality z; unfold Basics.compose.
+ f_equal; f_equal.
+ change (Z.of_nat 0 * 4)%Z with 0%Z. clear; omega.
+ pull_left   (array_at tuchar Tsh (ZnthV tuchar (map Vint dd'))
+            (Z.of_nat CBLOCK - 8) 60 (offset_val (Int.repr 40) c)) .
+ repeat rewrite sepcon_assoc.
+ apply sepcon_derives; [ | cancel_frame].
+ change 40%Z with (sizeof tuchar * 40)%Z at 1.
+ rewrite <- offset_val_array_at.
+ change (Int.repr 4) with (Int.repr (sizeof (tarray tuchar 4))).
+ rewrite memory_block_typed by reflexivity.
+ simpl_data_at.
+ change (40+56)%Z with (sizeof tuchar * (40+56))%Z.
+ rewrite <- offset_val_array_at.
+ change (40+56+4)%Z with (40+60)%Z.
+ change (40 + (Z.of_nat CBLOCK - 8))%Z with (40 + 56 + 0)%Z.
+ apply derives_refl'; apply equal_f; apply array_at_ext.
+ intros. unfold ZnthV. rewrite if_false by omega.
+ rewrite if_false by omega.
+ rewrite nth_overflow.
+ rewrite nth_overflow. auto.
+ simpl length.
+ rewrite Z2Nat.inj_sub by omega. omega.
+clear - H0 H9.
+ rewrite map_length in *.
+ change CBLOCK with 64%nat in H0.
+ assert (56 <= i-40)%Z by omega.
+ apply Z2Nat.inj_le in H; try omega.
+ change (Z.to_nat 56) with 56%nat in H; omega.
+ forward. (* p += 4; *)
+ entailer!.
+ forward. (* cNl=c->Nl; *)
+ forward. (* (void)HOST_l2c(cNl,p); *)
+ instantiate (1:=(offset_val (Int.repr 60) (offset_val (Int.repr 40) c),
+                         Tsh, lobytes)) in (Value of witness).
+ entailer!.
+ destruct c; try (contradiction Pc); simpl.
+ f_equal; repeat rewrite Int.add_assoc; f_equal.
+ unfold lobytes.
+ symmetry; rewrite (nth_big_endian_integer 0 [lo] lo) at 1 by reflexivity.
+ f_equal; extensionality z; unfold Basics.compose.
+ f_equal; f_equal.
+ change (Z.of_nat 0 * 4)%Z with 0%Z. clear; omega.
+ pull_left   (array_at tuchar Tsh (ZnthV tuchar (map Vint dd'))
+             60 64 (offset_val (Int.repr 40) c)) .
+ repeat rewrite sepcon_assoc.
+ apply sepcon_derives; [ | cancel_frame].
+ change 40%Z with (sizeof tuchar * 40)%Z at 1.
+ rewrite <- offset_val_array_at.
+ change (Int.repr 4) with (Int.repr (sizeof (tarray tuchar 4))).
+ rewrite memory_block_typed by reflexivity.
+ simpl_data_at.
+ change (40+60)%Z with (sizeof tuchar * (40+60))%Z.
+ rewrite <- offset_val_array_at.
+ change (40+60+0)%Z with (40+60)%Z.
+ change (40 + 60+4)%Z with (40 + 64)%Z.
+ apply derives_refl'; apply equal_f; apply array_at_ext.
+ intros. unfold ZnthV. rewrite if_false by omega.
+ rewrite if_false by omega.
+ rewrite nth_overflow.
+ rewrite nth_overflow. auto.
+ simpl length.
+ rewrite Z2Nat.inj_sub by omega. omega.
+clear - H0 H10.
+ rewrite map_length in *.
+ change CBLOCK with 64%nat in H0.
+ assert (60 <= i-40)%Z by omega.
+ apply Z2Nat.inj_le in H; try omega.
+ change (Z.to_nat 60) with 60%nat in H; omega.
+ autorewrite with subst.
+ normalize.
+ forward. (* p += 4; *)
+ entailer!. destruct c_; try (contradiction Pc_); apply I.
+ forward. (*   p -= SHA_CBLOCK; *)
+ entailer!. destruct c_; try (contradiction Pc_); apply I.
+ simpl. normalize.
+ simpl force_val2. normalize.
+ replace (array_at tuchar Tsh (cVint lobytes) 0 4) with 
+     (array_at tuchar Tsh  (ZnthV tuchar
+                (map Vint (map Int.repr (intlist_to_Zlist [lo])))) 0 4).
+Focus 2. apply array_at_ext; intros; unfold cVint, lobytes, ZnthV, Basics.compose; if_tac; try reflexivity.
+omega.
+rewrite (nth_map' Vint Vundef Int.zero)
+ by (simpl length; apply Nat2Z.inj_lt;
+       rewrite Z2Nat.id; change (Z.of_nat 4) with 4%Z; omega).
+ reflexivity.
+ replace (array_at tuchar Tsh (cVint hibytes) 0 4) with 
+     (array_at tuchar Tsh  (ZnthV tuchar
+                (map Vint (map Int.repr (intlist_to_Zlist [hi])))) 0 4).
+Focus 2. apply array_at_ext; intros; unfold cVint, hibytes, ZnthV, Basics.compose; if_tac; try reflexivity.
+omega.
+rewrite (nth_map' Vint Vundef Int.zero)
+ by (simpl length; apply Nat2Z.inj_lt;
+       rewrite Z2Nat.id; change (Z.of_nat 4) with 4%Z; omega).
+ reflexivity.
+clear lobytes hibytes.
+rewrite (Zlength_correct dd').
+rewrite (array_at_tuchar_isbyteZ _ dd').
+rewrite <- (Zlength_correct dd').
+normalize.
+rename H10 into Hforall; rewrite firstn_same in Hforall by (rewrite map_length; clear; omega).
+pose (lastblock := (
+         (dd' ++ zeros (Z.of_nat CBLOCK - 8 - Zlength dd')
+          ++  map Int.repr (intlist_to_Zlist [hi,lo])))).
+assert (H10: length lastblock = CBLOCK).
+unfold lastblock; repeat rewrite app_length.
+rewrite length_zeros; simpl.
+clear - H0.
+rewrite Zlength_correct. repeat rewrite Z2Nat.inj_sub by omega.
+repeat rewrite Nat2Z.id. rewrite map_length in H0. simpl Z.to_nat. omega.
+assert (BYTESlastblock: Forall isbyteZ (map Int.unsigned lastblock)). {
+ unfold lastblock.
+ repeat rewrite map_app.
+ repeat rewrite Forall_app.
+ repeat split; auto.
+ apply isbyte_zeros.
+ apply isbyte_intlist_to_Zlist'.
+}
+pose (lastblock' := Zlist_to_intlist (map Int.unsigned lastblock)).
+eapply semax_pre; [ | apply (sha_final_part3 Espec md c shmd hashed' lastblock'); auto].
+* entailer!.
+ + destruct c_; try (contradiction Pc_); simpl;
+     f_equal; rewrite Int.sub_add_opp;
+     repeat rewrite Int.add_assoc; f_equal; reflexivity.
+ + 
+unfold lastblock', data_block. (*rewrite map_swap_involutive.*)
+rewrite Zlist_to_intlist_to_Zlist; [ |rewrite map_length; rewrite H10; exists LBLOCK; reflexivity | assumption].
+rewrite Forall_isbyte_repr_unsigned.
+rewrite (Zlength_correct (map _ lastblock)). try rewrite map_length; rewrite H10.
+change (Z.of_nat CBLOCK) with 64%Z at 2.
+change (intlist_to_Zlist [hi, lo])
+  with (intlist_to_Zlist [hi] ++intlist_to_Zlist [lo]).
+apply (final_part5 hashed dd hashed' dd' pad (intlist_to_Zlist [hi]) (intlist_to_Zlist [lo]) hi lo);
+  auto.
+* unfold lastblock'.
+apply length_Zlist_to_intlist.
+rewrite map_length; assumption.
+*
+apply intlist_to_Zlist_inj.
+rewrite (lastblock_lemma _ hashed' (map Int.unsigned dd') pad hi lo); auto.
+2: destruct PAD as [PAD|PAD];[left|right]; rewrite PAD; reflexivity.
+2: repeat rewrite app_ass; apply H5.
+rewrite (app_ass _ (map Int.unsigned dd)); rewrite <- H5.
+rewrite app_ass; rewrite intlist_to_Zlist_app.
+f_equal.
+unfold lastblock'.
+rewrite Zlist_to_intlist_to_Zlist; auto.
+2:  rewrite map_length, H10; eexists;reflexivity.
+unfold lastblock; repeat rewrite map_app.
+f_equal.
+f_equal.
+f_equal.
+f_equal.
+admit.
+rewrite <- H7; f_equal.
+rewrite initial_world.Zlength_app, initial_world.Zlength_map.
+rewrite Zlength_intlist_to_Zlist.
+rewrite Z.mul_comm; reflexivity.
+rewrite Forall_app; split; [apply isbyte_intlist_to_Zlist | ].
+  assert (Forall isbyteZ (intlist_to_Zlist hashed' ++ map Int.unsigned dd' )).
+rewrite Forall_app; split; [apply isbyte_intlist_to_Zlist | auto].
+rewrite H5 in H11.
+clear - H11; repeat rewrite Forall_app in H11; intuition.
+Qed.
