progs/verif_sha_init.v
@@ -3,6 +3,7 @@ Require Import progs.sha.
 Require Import progs.SHA256.
 Require Import progs.sha_lemmas.
 Require Import progs.spec_sha.
+Local Open Scope nat.
 Local Open Scope logic.
 
 Lemma ZnthV_nil_None:
